well formed contexts are a pain

theories/LogicalRelation/Definition/Bool.v
@@ -11,7 +11,7 @@ Set Polymorphic Inductive Cumulativity.
 (** ** Reducibility of boolean type *)
 Module BoolRedTy.
 
-  Record SBoolRedTy `{ta : tag} `{WfType ta} `{RedType ta}
+  Record BoolRedTy `{ta : tag} `{WfType ta} `{RedType ta}
     {Γ : context} {A B : term}
   : Set :=
   {
@@ -19,30 +19,30 @@ Module BoolRedTy.
     redR : [Γ |- B :⤳*: tBool]
   }.
 
-  Arguments SBoolRedTy {_ _ _}.
+  Arguments BoolRedTy {_ _ _}.
 
-  Definition BoolRedTy `{ta : tag} `{WfType ta} `{RedType ta} : forall Γ A B, Type :=
-    Split_Rel SBoolRedTy.
+  Definition shfBoolRedTy `{ta : tag} `{WfType ta} `{RedType ta} : forall Γ A B, Type :=
+    Split_Rel BoolRedTy.
 
   Section BoolRedTy.
   Context `{ta : tag} `{WfType ta} `{RedType ta}.
 
-  Definition whredL {Γ A B} : SBoolRedTy Γ A B -> [Γ |- A ↘].
+  Definition whredL {Γ A B} : BoolRedTy Γ A B -> [Γ |- A ↘].
   Proof. intros []; econstructor; tea; constructor. Defined.
 
-  Definition whredR {Γ A B} : SBoolRedTy Γ A B -> [Γ |- B ↘].
+  Definition whredR {Γ A B} : BoolRedTy Γ A B -> [Γ |- B ↘].
   Proof. intros []; econstructor; tea; constructor. Defined.
 
   End BoolRedTy.
 
 End BoolRedTy.
 
-Export BoolRedTy(SBoolRedTy, BoolRedTy, Build_SBoolRedTy).
-Notation "[ Γ ||-SBool A ≅ B ]" := (SBoolRedTy Γ A B) (at level 0, Γ, A at level 50).
+Export BoolRedTy(BoolRedTy, shfBoolRedTy, Build_BoolRedTy).
+Notation "[ Γ ||-shfBool A ≅ B ]" := (shfBoolRedTy Γ A B) (at level 0, Γ, A at level 50).
 Notation "[ Γ ||-Bool A ≅ B ]" := (BoolRedTy Γ A B) (at level 0, Γ, A at level 50).
 
 #[program]
-Instance WhRedTyBoolRedTy `{GenericTypingProperties} {Γ} : WhRedTyRel Γ (SBoolRedTy Γ) :=
+Instance WhRedTyBoolRedTy `{GenericTypingProperties} {Γ} : WhRedTyRel Γ (BoolRedTy Γ) :=
   {|
     whredtyL := fun A B RAB => BoolRedTy.whredL RAB ;
     whredtyR := fun A B RAB => BoolRedTy.whredR RAB ;
@@ -64,7 +64,7 @@ Section BoolRedTmEq.
   | neReq {ne ne'} : [Γ ||-NeNf ne ≅ ne' : tBool] -> BoolPropEq Γ ne ne'.
 
 
-  Record SBoolRedTmEq {Γ t u} : Set :=
+  Record BoolRedTmEq {Γ t u} : Set :=
     {
       nfL : term ;
       nfR : term ;
@@ -73,10 +73,10 @@ Section BoolRedTmEq.
       eq : [Γ |- nfL ≅ nfR : tBool] ;
       prop : BoolPropEq Γ nfL nfR
   }.
-  Arguments SBoolRedTmEq : clear implicits.
+  Arguments BoolRedTmEq : clear implicits.
 
-  Definition BoolRedTmEq : forall Γ t u, Set :=
-    Split_Rel SBoolRedTmEq.
+  Definition shfBoolRedTmEq : forall Γ t u, Set :=
+    Split_Rel BoolRedTmEq.
 
   Section Def.
     Context `{!GenericTypingProperties _ _ _ _ _ _ _ _ _}.
@@ -94,12 +94,12 @@ Section BoolRedTmEq.
     Definition whnfR {Γ t u} : BoolPropEq Γ t u -> whnf u.
     Proof. intros []%BoolPropEq_isBool; now eapply isBool_whnf. Qed.
 
-    Definition whredL {Γ t u} : SBoolRedTmEq Γ t u -> [Γ |- t ↘ tBool].
+    Definition whredL {Γ t u} : BoolRedTmEq Γ t u -> [Γ |- t ↘ tBool].
     Proof.
       intros []; econstructor; tea; now eapply whnfL.
     Defined.
 
-    Definition whredR {Γ t u} : SBoolRedTmEq Γ t u -> [Γ |- u ↘ tBool].
+    Definition whredR {Γ t u} : BoolRedTmEq Γ t u -> [Γ |- u ↘ tBool].
     Proof.
       intros []; econstructor; tea; now eapply whnfR.
     Defined.
@@ -109,17 +109,17 @@ Section BoolRedTmEq.
 
 End BoolRedTmEq.
 Arguments BoolPropEq {_ _ _}.
-Arguments SBoolRedTmEq {_ _ _ _ _}.
+Arguments shfBoolRedTmEq {_ _ _ _ _}.
 Arguments BoolRedTmEq {_ _ _ _ _}.
 End BoolRedTmEq.
 
-Export BoolRedTmEq(BoolRedTmEq,SBoolRedTmEq,Build_SBoolRedTmEq,BoolPropEq,BoolPropEq_isBool).
+Export BoolRedTmEq(BoolRedTmEq,shfBoolRedTmEq,Build_BoolRedTmEq,BoolPropEq,BoolPropEq_isBool).
 
-Notation "[ Γ ||-SBool t ≅ u :Bool]" := (@SBoolRedTmEq _ _ _ _ _ _ _ Γ t u).
+Notation "[ Γ ||-shfBool t ≅ u :Bool]" := (@shfBoolRedTmEq _ _ _ _ _ _ _ Γ t u).
 Notation "[ Γ ||-Bool t ≅ u :Bool]" := (@BoolRedTmEq _ _ _ _ _ _ _ Γ t u).  (* (at level 0, Γ, t, u at level 50). *)
 
 #[program]
-Instance BoolRedTmEqWhRed `{GenericTypingProperties} {Γ} : WhRedTmRel Γ tBool (SBoolRedTmEq Γ) :=
+Instance BoolRedTmEqWhRed `{GenericTypingProperties} {Γ} : WhRedTmRel Γ tBool (BoolRedTmEq Γ) :=
   {| whredtmL := fun t u Rtu => BoolRedTmEq.whredL Rtu ;
     whredtmR := fun t u Rtu => BoolRedTmEq.whredR Rtu |}.
 Next Obligation.
