theories/LogicalRelation/Weakening.v
@@ -16,17 +16,17 @@ Section Weakenings.
   Record kripke@{i j k l} {Γ l A B} {RAB : [LogRel@{i j k l} l | Γ ||- A ≅ B]} := {
     wkRed : forall {Δ} (ρ : Δ ≤ Γ) (wfΔ : [|-Δ]), [LogRel@{i j k l} l | Δ ||- A⟨ρ⟩ ≅ B⟨ρ⟩] ;
     wkRedTm : forall {Δ} (ρ : Δ ≤ Γ) (wfΔ : [|-Δ]) {t u},
-      [Γ ||-<l> t ≅ u : _ | RAB] -> [Δ ||-<l> t⟨ρ⟩ ≅ u⟨ρ⟩ : _ | wkRed ρ wfΔ] ;
+      [Γ ||-S<l> t ≅ u : _ | RAB] -> [Δ ||-S<l> t⟨ρ⟩ ≅ u⟨ρ⟩ : _ | wkRed ρ wfΔ] ;
   }.
   Arguments kripke {_ _ _ _} _.
 
   Definition wkStmt@{i j k l} l := (forall Γ A B (R : [LogRel@{i j k l} l | Γ ||- A ≅ B]), kripke R).
 
-  Lemma wkU {Γ Δ l A B} (ρ : Δ ≤ Γ) (wfΔ : [|-Δ]) (h : [Γ ||-SU<l> A ≅ B]) : [Δ ||-SU<l> A⟨ρ⟩ ≅ B⟨ρ⟩].
+  Lemma wkU {Γ Δ l A B} (ρ : Δ ≤ Γ) (wfΔ : [|-Δ]) (h : [Γ ||-U<l> A ≅ B]) : [Δ ||-U<l> A⟨ρ⟩ ≅ B⟨ρ⟩].
   Proof. destruct h; econstructor; tea; change U with U⟨ρ⟩; gen_typing. Defined.
 
   Lemma wkURedTerm {Γ Δ l t} (ρ : Δ ≤ Γ) (wfΔ : [|-Δ]) :
-    SURedTm l Γ t -> SURedTm l Δ t⟨ρ⟩.
+    URedTm l Γ t -> URedTm l Δ t⟨ρ⟩.
   Proof.
     intros [te]. exists te⟨ρ⟩; change U with U⟨ρ⟩.
     - gen_typing.
@@ -35,7 +35,7 @@ Section Weakenings.
 
   Lemma wkLRU {l}
     (ih : forall l', l' << l -> wkStmt l')
-    {Γ A B} {h : [Γ ||-SU<l> A ≅ B]} : kripke (LRU_ h).
+    {Γ A B} {h : [Γ ||-U<l> A ≅ B]} : kripke (LRU_ h).
   Proof.
     unshelve econstructor.
     1: intros; now eapply LRU_, wkU.
@@ -55,7 +55,7 @@ Section Weakenings.
     intros []; opector.
     - intros ? ρ' ?; rewrite 2!wk_comp_ren_on; now eapply shpRed.
     - intros ? a b ρ' **; rewrite <-2!wk_up_ren_subst.
-      unshelve eapply posRed; tea; eapply irrLREq; tea; now rewrite wk_comp_ren_on.
+      unshelve eapply posRed; tea; eapply SirrLREq; tea; now rewrite wk_comp_ren_on.
   Qed.
 
   Lemma wkParamTy {T Γ A shp pos Δ} (ρ : Δ ≤ Γ) (wfΔ : [|-Δ])
@@ -95,11 +95,11 @@ Section Weakenings.
     + now eapply convty_wk.
     + intros Ξ a b ρΞ wfΞ *; cbn in *.
       eassert ([_ |_||- _≅ _ : (ParamRedTy.domL ΠA)⟨ρΞ∘w ρ⟩ ≅ _]) as ha'
-        by (eapply irrLREq; [eapply wk_comp_ren_on| eapply ha]).
+        by (eapply SirrLREq; [eapply wk_comp_ren_on| eapply ha]).
       specialize (Ht _ _ _ (ρΞ∘w ρ) wfΞ ha').
       eapply (dSplit_bind_return_over Ht).
-      intros Θ ρΘ hovera' hovert hoverwk; cbn in *.
-      rewrite <-2!wk_up_ren_subst ; eapply irrLREq.
+      intros Θ ρΘ hovera' hovert hoverwk hΘ; cbn in *.
+      rewrite <-2!wk_up_ren_subst ; eapply SirrLREq.
       1: now rewrite <-wk_up_ren_subst.
       unshelve eapply Ht; tea.
     + cbn; rewrite wk_prod; now eapply convneu_wk.
@@ -123,11 +123,11 @@ Section Weakenings.
       1: cbn; rewrite wk_prod; now eapply convtm_wk.
       intros Ξ a b ρΞ wfΞ hab; cbn in *; rewrite 2!wk_comp_ren_on.
       eassert ([_ |_||- _≅ _ : (ParamRedTy.domL ΠA)⟨ρΞ∘w ρ⟩ ≅ _]) as hab'
-        by (eapply irrLREq; [eapply wk_comp_ren_on| eapply hab]).
+        by (eapply SirrLREq; [eapply wk_comp_ren_on| eapply hab]).
       specialize (eqApp Ξ a b (ρΞ∘w ρ) wfΞ hab').
       eapply (dSplit_bind_return_over eqApp).
-      intros Θ ρΘ hoverab' hovereqApp hoverwk.
-      eapply irrLREq; [now rewrite <-wk_up_ren_subst| unshelve eapply eqApp; tea].
+      intros Θ ρΘ hoverab' hovereqApp hoverwk hΘ.
+      eapply SirrLREq; [now rewrite <-wk_up_ren_subst| unshelve eapply eqApp; tea].
   Qed.
 
   Lemma wk_up_subst1 {Γ Δ F} t a (ρ : Γ ≤ Δ) : t⟨wk_up F ρ⟩[(a⟨ρ⟩)..] = t[a..]⟨ρ⟩.
@@ -139,7 +139,7 @@ Section Weakenings.
   intros * [A' B' a b wtydom convtydom wtycod convtycod Hfst Hsnd|]; unshelve econstructor; tea; refold.
   all: try first [now eapply wft_wk| now eapply convty_wk].
   + refold; intros Ξ ρ' wfΞ.
-    rewrite wk_comp_ren_on; eapply irrLREq; [|now unshelve eapply Hfst].
+    rewrite wk_comp_ren_on; eapply SirrLREq; [|now unshelve eapply Hfst].
     cbn; now rewrite wk_comp_ren_on.
   + erewrite <- (wk_up_ren_on _ _ _ A'), wk_up_subst1.
     now eapply wft_wk.
@@ -148,8 +148,8 @@ Section Weakenings.
   + refold; intros Ξ ρΞ wfΞ.
     specialize (Hsnd Ξ (ρΞ ∘w ρ) wfΞ).
     eapply (dSplit_bind_return_over Hsnd).
-    intros Θ ρΘ hoverfst hoversnd hover.
-    eapply irrLREq; clear hover.
+    intros Θ ρΘ hoverfst hoversnd hover hΘ.
+    eapply SirrLREq; clear hover.
     2:rewrite (wk_comp_ren_on b); now unshelve apply Hsnd.
     cbn; now rewrite <-wk_up_ren_subst, wk_comp_ren_on.
   + cbn; rewrite wk_sig; now eapply convneu_wk.
@@ -172,36 +172,36 @@ Section Weakenings.
       1,2: now apply wkSigRedTerm.
       2: cbn; rewrite wk_sig; now eapply convtm_wk.
       + intros Ξ ρ' wfΞ ; cbn; rewrite 2!wk_comp_ren_on.
-        eapply irrLREq; [now rewrite wk_comp_ren_on| now unshelve eapply eqFst].
+        eapply SirrLREq; [now rewrite wk_comp_ren_on| now unshelve eapply eqFst].
       + intros Ξ ρΞ wfΞ ; cbn.
         specialize (eqSnd Ξ (ρΞ∘w ρ) wfΞ).
         eapply (dSplit_bind_return_over eqSnd).
-        intros Θ ρΘ hoverFst hoverSnd hover; cbn in *.
-        eapply irrLREq; clear hover.
+        intros Θ ρΘ hoverFst hoverSnd hover hΘ; cbn in *.
+        eapply SirrLREq; clear hover.
         2: rewrite 2!wk_comp_ren_on; now unshelve eapply eqSnd.
         cbn; now rewrite <-wk_up_ren_subst, wk_comp_ren_on.
   Qed.
 
-  Lemma wkNat {Γ A B Δ} (ρ : Δ ≤ Γ) (wfΔ : [|- Δ]) : [Γ ||-SNat A ≅ B] -> [Δ ||-SNat A⟨ρ⟩ ≅ B⟨ρ⟩].
+  Lemma wkNat {Γ A B Δ} (ρ : Δ ≤ Γ) (wfΔ : [|- Δ]) : [Γ ||-Nat A ≅ B] -> [Δ ||-Nat A⟨ρ⟩ ≅ B⟨ρ⟩].
   Proof.
     intros []; constructor.
     all: change tNat with tNat⟨ρ⟩; gtyping.
   Qed.
 
-  Lemma wkBool {Γ A B Δ} (ρ : Δ ≤ Γ) (wfΔ : [|- Δ]) : [Γ ||-SBool A ≅ B] -> [Δ ||-SBool A⟨ρ⟩ ≅ B⟨ρ⟩].
+  Lemma wkBool {Γ A B Δ} (ρ : Δ ≤ Γ) (wfΔ : [|- Δ]) : [Γ ||-Bool A ≅ B] -> [Δ ||-Bool A⟨ρ⟩ ≅ B⟨ρ⟩].
   Proof.
     intros []; constructor.
     all: change tBool with tBool⟨ρ⟩; gtyping.
   Qed.
 
-  Lemma wkEmpty {Γ A B Δ} (ρ : Δ ≤ Γ) (wfΔ : [|- Δ]) : [Γ ||-SEmpty A ≅ B] -> [Δ ||-SEmpty A⟨ρ⟩ ≅ B⟨ρ⟩].
+  Lemma wkEmpty {Γ A B Δ} (ρ : Δ ≤ Γ) (wfΔ : [|- Δ]) : [Γ ||-Empty A ≅ B] -> [Δ ||-Empty A⟨ρ⟩ ≅ B⟨ρ⟩].
   Proof.
     intros []; constructor; change tEmpty with tEmpty⟨ρ⟩; gtyping.
   Qed.
 
-  Lemma wkId@{i j k l} {Γ l A B} (IA : SIdRedTy@{i j k l} Γ l A B)
+  Lemma wkId@{i j k l} {Γ l A B} (IA : IdRedTy@{i j k l} Γ l A B)
     (ih : kripke@{i j k l} IA.(IdRedTy.tyRed)) {Δ} (ρ : Δ ≤ Γ) (wfΔ : [|- Δ]) :
-    SIdRedTy@{i j k l} Δ l A⟨ρ⟩ B⟨ρ⟩.
+    IdRedTy@{i j k l} Δ l A⟨ρ⟩ B⟨ρ⟩.
   Proof.
     unshelve econstructor.
     8,9: erewrite wk_Id; eapply redtywf_wk; tea; apply IA.(IdRedTy.redL) + apply IA.(IdRedTy.redR).
@@ -209,7 +209,7 @@ Section Weakenings.
     - now eapply ih.(wkRed).
     - eapply wkRedTm; now destruct IA.
     - eapply wkRedTm; now destruct IA.
-    - apply perLRTm.
+    - eapply SperLRTm.
   Defined.
 
   Lemma wkNeNfEq {Γ Δ k k' A} (ρ : Δ ≤ Γ) (wfΔ : [|-Δ]) :
@@ -236,25 +236,15 @@ Section Weakenings.
       + intros; now eapply LRNat_, wkNat.
       + intros ??? t u hNat; cbn in *. revert t u hNat Δ ρ wfΔ.
         set (G := _); enough (h : G ×
-          (forall t u, NatRedTmEq Γ t u -> forall Δ (ρ : Δ ≤ Γ), [ |-[ ta ] Δ] -> NatRedTmEq Δ t⟨ρ⟩ u⟨ρ⟩) ×
           (forall t u, NatPropEq Γ t u -> forall Δ (ρ : Δ ≤ Γ), [ |-[ ta ] Δ] ->NatPropEq Δ t⟨ρ⟩ u⟨ρ⟩))
           by apply h.
-        subst G; clear NA; revert Γ; apply NatRedEqInduction with 
-          (P:= fun Γ t u _ => forall Δ (ρ : Δ ≤ Γ), [ |-[ ta ] Δ] -> [Δ ||-SNat t⟨ρ⟩ ≅ u⟨ρ⟩:Nat])
-          (P1:= fun Γ t u _ => forall Δ (ρ : Δ ≤ Γ), [ |-[ ta ] Δ] -> [Δ ||-Nat t⟨ρ⟩ ≅ u⟨ρ⟩:Nat])
-          (P0:= fun Γ t u _ => forall Δ (ρ : Δ ≤ Γ), [ |-[ ta ] Δ] -> NatPropEq Δ t⟨ρ⟩ u⟨ρ⟩).
-        * intros; econstructor; tea; change tNat with tNat⟨ρ⟩; gtyping.
+        subst G; apply NatRedEqInduction.
+        * intros; econstructor; tea; change tNat with tNat⟨ρ⟩; gen_typing.
         * constructor.
         * now constructor.
         * intros; constructor.
           change tNat with tNat⟨ρ⟩.
           now eapply wkNeNfEq.
-        * intros ???? htu ihtu Δ ρ hΔ.
-          econstructor.
-          intros Ξ ρΞ hover.
-          rewrite 2!wk_comp_ren_on.
-          eapply htu.
-          now eapply over_DTree_PSh.
     - intros; unshelve econstructor.
       + intros; now apply LRBool_, wkBool.
       + cbn; intros ????? [ ]; econstructor; change tBool with tBool⟨ρ⟩.
