theories/LogicalRelation/Definition/Pi.v
@@ -27,8 +27,8 @@ Inductive isLRFun `{ta : tag} `{WfContext ta}
     [Γ |-  ΠA.(PiRedTyPack.domL) ≅ A'] ->
     (forall {Δ a b} (ρ : Δ ≤ Γ) (h : [ |- Δ ])
       (ha : [ ΠA.(PolyRedPack.shpRed) ρ h | Δ ||- a ≅ b : ΠA.(PiRedTyPack.domL)⟨ρ⟩ ]),
-        dSplit (fun Ξ ρ' hSplit => 
-          [hSplit | Ξ ||- t[a .: (ρ >> tRel)]⟨ρ'⟩ ≅ t[b .: (ρ >> tRel)]⟨ρ'⟩ : ΠA.(PiRedTyPack.codL)[a .: (ρ >> tRel)]⟨ρ'⟩])
+        dSplit (fun Ξ ρ' hSplit => forall (hΞ : [|-Ξ]),
+          [hSplit hΞ | Ξ ||- t[a .: (ρ >> tRel)]⟨ρ'⟩ ≅ t[b .: (ρ >> tRel)]⟨ρ'⟩ : ΠA.(PiRedTyPack.codL)[a .: (ρ >> tRel)]⟨ρ'⟩])
         (ΠA.(PolyRedPack.posRed) ρ h ha)) ->
   isLRFun ΠA (tLambda A' t)
 | NeLRFun : forall f : term, [Γ |- f ~ f : PiRedTyPack.outTy ΠA] -> isLRFun ΠA f.
@@ -41,7 +41,7 @@ Module PiRedTmEq.
     {Γ A B} (ΠA : PiRedTyPack Γ A B) (nfL nfR : term) Δ a b :=
     forall (ρ : Δ ≤ Γ) (h : [ |- Δ ])
       (hab : [ΠA.(PolyRedPack.shpRed) (ρ) h | Δ ||- a ≅ b : ΠA.(domL)⟨ρ⟩]),
-      dSplit (fun Ξ ρ' hSplit => [ hSplit | Ξ ||- (tApp nfL⟨ρ⟩ a)⟨ρ'⟩ ≅ (tApp nfR⟨ρ⟩ b)⟨ρ'⟩ : _ ]) (ΠA.(PolyRedPack.posRed) ρ h hab).
+      dSplit (fun Ξ ρ' hSplit => forall hΞ :[|-Ξ], [ hSplit hΞ | Ξ ||- (tApp nfL⟨ρ⟩ a)⟨ρ'⟩ ≅ (tApp nfR⟨ρ⟩ b)⟨ρ'⟩ : _ ]) (ΠA.(PolyRedPack.posRed) ρ h hab).
 
   Arguments appRed /.
 
