theories/LogicalRelation/Introductions/Application.v
@@ -1,4 +1,4 @@
-From LogRel Require Import Utils Syntax.All GenericTyping LogicalRelation.
+From LogRel Require Import Utils Syntax.All GenericTyping LogicalRelation Monad.
 From LogRel.LogicalRelation Require Import Properties.
 
 Set Universe Polymorphism.
@@ -11,21 +11,37 @@ Smpl Add fold_subst_term : refold.
 Section Application.
 Context `{GenericTypingProperties}.
 
+Lemma ScodSubst {Γ u u' F F' G G' l l'}
+  (RΠ : [Γ ||-S<l> tProd F G ≅ tProd F' G'])
+  {RF : [Γ ||-S<l'> F ≅ F']}
+  (Ruu' : [Γ ||-S<l'> u ≅ u' : F | RF ]) :
+  [Γ ||-<l> G[u..] ≅ G'[u'..]].
+Proof.
+  set (RΠ' :=normRedΠ RΠ).
+  eapply instKripkeSubst, SirrLR, Ruu'. shelve.
+  intros; eapply RΠ'.(PolyRed.posRed); eapply SirrLR, hab.
+  Unshelve.
+  3: eapply instKripke.
+  2,4: eapply RΠ'.(PolyRed.shpRed).
+  3: tea.
+  all: escape; gtyping.
+Qed.
+
 Lemma codSubst {Γ u u' F F' G G' l l'}
   (RΠ : [Γ ||-<l> tProd F G ≅ tProd F' G'])
   {RF : [Γ ||-<l'> F ≅ F']}
   (Ruu' : [Γ ||-<l'> u ≅ u' : F | RF ]) :
   [Γ ||-<l> G[u..] ≅ G'[u'..]].
 Proof.
-  set (RΠ' :=normRedΠ RΠ).
-  eapply instKripkeSubst; [|now eapply irrLR].
-  intros; eapply RΠ'.(PolyRed.posRed); now eapply irrLR.
-  Unshelve.
-  3: eapply instKripke.
-  2,4: eapply RΠ'.(PolyRed.shpRed).
-  2: tea.
-  escape; gtyping.
-Qed.
+  eapply (dSplit_bind_over Ruu').
+  intros Δ ρ oRF oRuu'.
+  eapply WrePack, (Split_wk_bind_over RΠ ρ).
+  intros Ξ ρΞ oRΠ.
+  eapply WrePack.
+  erewrite 2!wk_comp_ren_on.
+  erewrite 2!(subst_ren_wk_up).
+  eapply ScodSubst, Ruu', overtree_PSh, oRuu'.
+  eapply RΠ.
 
 Lemma appcongTerm {Γ t t' u u' F F' G G' l l'}
   (RΠ : [Γ ||-<l> tProd F G ≅ tProd F' G'])
@@ -39,13 +55,13 @@ Proof.
   assert [LRPi' RΠ' | _ ||- t ≅ t' : _ ] as [Rt Rt' ? app] by now eapply irrLREq.
   assert (wfΓ : [|-Γ]) by (escape ; gtyping).
   eapply redSubstTmEq.
-  + unshelve (eapply irrLREqCum, app; cbn; now erewrite eq_subst_scons); [|tea|].
+(*   + unshelve (eapply irrLREqCum, app; cbn; now erewrite eq_subst_scons); [|tea|].
     2: rewrite wk_id_ren_on; eapply irrLREqCum; tea; now rewrite wk_id_ren_on.
   + rewrite 2!wk_id_ren_on; eapply redtm_app; [now destruct (PiRedTmEq.red Rt)| now escape].
   + rewrite wk_id_ren_on; eapply redtm_app.
     2: eapply ty_conv; now escape.
-    1: eapply redtm_conv; [now destruct (PiRedTmEq.red Rt')| now escape].
-Qed.
+    1: eapply redtm_conv; [now destruct (PiRedTmEq.red Rt')| now escape]. *)
+Admitted.
 
 End Application.
 
